compiler/backend/proofs/bvp_to_wordProofScript.sml
@@ -3069,7 +3069,7 @@ val get_real_offset_thm = store_thm("get_real_offset_thm",
   fs [labPropsTheory.good_dimindex_def,dimword_def] \\ rw []
   \\ fs [get_real_offset_def,bytes_in_word_def,word_mul_n2w,WORD_MUL_LSL]);
 
-val memory_rel_El = prove(
+val memory_rel_El = store_thm("memory_rel_El",
   ``memory_rel c be refs sp st m dm
      ((Block tag vals,ptr)::(Number (&index),i)::vars) /\
     good_dimindex (:'a) /\
@@ -3122,7 +3122,7 @@ val memory_rel_El = prove(
   \\ fs [word_list_def,word_list_APPEND]
   \\ SEP_R_TAC \\ fs []);
 
-val memory_rel_Deref = prove(
+val memory_rel_Deref = store_thm("memory_rel_Deref",
   ``memory_rel c be refs sp st m dm
      ((RefPtr nn,ptr)::(Number (&index),i)::vars) /\
     FLOOKUP refs nn = SOME (ValueArray vals) /\
@@ -3182,7 +3182,7 @@ val memory_rel_Deref = prove(
   \\ fs [word_list_def,word_list_APPEND,SEP_CLAUSES] \\ fs [SEP_F_def]
   \\ SEP_R_TAC \\ fs []);
 
-val memory_rel_Update = prove(
+val memory_rel_Update = store_thm("memory_rel_Update",
   ``memory_rel c be refs sp st m dm
      ((h,w)::(RefPtr nn,ptr)::(Number (&index),i)::vars) /\
     FLOOKUP refs nn = SOME (ValueArray vals) /\
@@ -3275,7 +3275,7 @@ val bytes_in_word_mul_eq_shift = store_thm("bytes_in_word_mul_eq_shift",
 val encode_header_IMP = prove(
   ``encode_header c tag len = SOME (hd:'a word) ==>
     len < 2 ** (dimindex (:'a) - 4) /\
-    decode_header c hd = (n2w tag << 2,n2w len)``,
+    decode_header c hd = (n2w tag,n2w len)``,
   fs [encode_header_def] \\ rw [decode_header_def]
   \\ cheat (* annoying word proofs *));
 
@@ -3294,10 +3294,10 @@ val EVERY2_f_EQ = prove(
   ``!rs ws f. EVERY2 (\v w. f v = w) rs ws <=> MAP f rs = ws``,
   Induct \\ fs [] \\ rw [] \\ eq_tac \\ rw [] \\ fs []);
 
-val memory_rel_Cons = prove(
+val memory_rel_Cons = store_thm("memory_rel_Cons",
   ``memory_rel c be refs sp st m dm (ZIP (vals,ws) ++ vars) /\
     LENGTH vals = LENGTH (ws:'a word_loc list) /\ vals <> [] /\
-    encode_header c tag (LENGTH ws) = SOME hd /\
+    encode_header c (4 * tag) (LENGTH ws) = SOME hd /\
     LENGTH ws < sp /\ good_dimindex (:'a) ==>
     ?eoh (curr:'a word) m1.
       FLOOKUP st EndOfHeap = SOME (Word eoh) /\
@@ -3344,7 +3344,70 @@ val memory_rel_Cons = prove(
          SEP_CLAUSES,word_heap_heap_expand]
   \\ fs [word_list_exists_ADD |> Q.SPECL [`m`,`n+1`]]
   \\ `(n2w tag ≪ (c.len_size + 4) ‖ n2w (LENGTH ws) ≪ 2 ‖ 3w) = hd` by
-       (fs [encode_header_def] \\ every_case_tac \\ fs [] \\ NO_TAC)
+       (fs [encode_header_def] \\ every_case_tac \\ fs []
+        \\ fs [WORD_MUL_LSL,word_mul_n2w,EXP_ADD] \\ NO_TAC)
+  \\ fs [] \\ imp_res_tac encode_header_IMP
+  \\ simp [WORD_MUL_LSL,word_mul_n2w]
+  \\ fs [SEP_CLAUSES,STAR_ASSOC]
+  \\ `LENGTH ws + 1 = LENGTH (Word hd::ws)` by fs []
+  \\ full_simp_tac std_ss []
+  \\ assume_tac store_list_thm
+  \\ SEP_F_TAC \\ strip_tac \\ fs []
+  \\ fs [EVERY2_f_EQ] \\ clean_tac \\ fs []
+  \\ fs [el_length_def,heap_length_APPEND,heap_length_heap_expand,
+         GSYM word_add_n2w,WORD_LEFT_ADD_DISTRIB]
+  \\ fs [AC STAR_ASSOC STAR_COMM] \\ fs [STAR_ASSOC]
+  \\ pop_assum mp_tac \\ CONV_TAC (DEPTH_CONV ETA_CONV)
+  \\ fs [AC STAR_ASSOC STAR_COMM] \\ fs [STAR_ASSOC]);
+
+val memory_rel_Ref = store_thm("memory_rel_Ref",
+  ``memory_rel c be refs sp st m dm (ZIP (vals,ws) ++ vars) /\
+    LENGTH vals = LENGTH (ws:'a word_loc list) /\ vals <> [] /\
+    encode_header c 2 (LENGTH ws) = SOME hd /\ ~(new IN FDOM refs) /\
+    LENGTH ws < sp /\ good_dimindex (:'a) ==>
+    ?eoh (curr:'a word) m1.
+      FLOOKUP st EndOfHeap = SOME (Word eoh) /\
+      FLOOKUP st CurrHeap = SOME (Word curr) /\
+      let w = eoh - bytes_in_word * n2w (LENGTH ws + 1) in
+        store_list w (Word hd::ws) m dm = SOME m1 /\
+        memory_rel c be (refs |+ (new,ValueArray vals)) (sp - (LENGTH ws + 1))
+          (st |+ (EndOfHeap,Word w)) m1 dm
+          ((RefPtr new,make_ptr c (w - curr) tag (LENGTH ws))::vars)``,
+  simp_tac std_ss [LET_THM]
+  \\ rewrite_tac [CONJ_ASSOC]
+  \\ once_rewrite_tac [CONJ_COMM]
+  \\ fs [memory_rel_def,PULL_EXISTS] \\ rw []
+  \\ fs [word_ml_inv_def,PULL_EXISTS] \\ clean_tac
+  \\ fs [MAP_ZIP]
+  \\ drule (GEN_ALL new_ref_thm)
+  \\ disch_then (qspecl_then [`Word 0w`,`new`] strip_assume_tac)
+  \\ rfs [] \\ fs [] \\ clean_tac
+  \\ rewrite_tac [GSYM CONJ_ASSOC]
+  \\ once_rewrite_tac [METIS_PROVE [] ``b1 /\ b2 /\ b3 <=> b2 /\ b1 /\ b3:bool``]
+  \\ drule pop_thm \\ fs []
+  \\ strip_tac \\ asm_exists_tac \\ fs [word_addr_def]
+  \\ fs [heap_in_memory_store_def,FLOOKUP_UPDATE]
+  \\ imp_res_tac heap_store_unused_IMP_length \\ fs []
+  \\ `LENGTH ws + 1 <= sp'` by decide_tac
+  \\ pop_assum mp_tac \\ simp_tac std_ss [LESS_EQ_EXISTS]
+  \\ strip_tac \\ clean_tac \\ fs []
+  \\ fs [GSYM word_add_n2w,WORD_LEFT_ADD_DISTRIB]
+  \\ fs [copying_gcTheory.EVERY2_APPEND]
+  \\ fs [WORD_LEFT_ADD_DISTRIB,get_addr_def,make_ptr_def,get_lowerbits_def]
+  \\ fs [bytes_in_word_mul_eq_shift]
+  \\ fs [GSYM bytes_in_word_mul_eq_shift,GSYM word_add_n2w]
+  \\ fs [heap_store_unused_def,el_length_def]
+  \\ every_case_tac \\ fs []
+  \\ imp_res_tac heap_lookup_SPLIT \\ fs [] \\ clean_tac
+  \\ full_simp_tac std_ss [APPEND,GSYM APPEND_ASSOC]
+  \\ fs [heap_store_lemma] \\ clean_tac \\ fs []
+  \\ fs [word_heap_APPEND,word_heap_def,word_el_def,word_payload_def,
+         SEP_CLAUSES,word_heap_heap_expand,RefBlock_def,el_length_def,
+         heap_length_APPEND,heap_length_heap_expand]
+  \\ fs [word_list_exists_ADD |> Q.SPECL [`m`,`n+1`]]
+  \\ `(n2w (LENGTH ws) ≪ 2 ‖ 2w ≪ (c.len_size + 2) ‖ 3w) = hd` by
+       (fs [encode_header_def] \\ every_case_tac \\ fs []
+        \\ fs [WORD_MUL_LSL,word_mul_n2w,EXP_ADD] \\ NO_TAC)
   \\ fs [] \\ imp_res_tac encode_header_IMP
   \\ fs [SEP_CLAUSES,STAR_ASSOC]
   \\ `LENGTH ws + 1 = LENGTH (Word hd::ws)` by fs []
@@ -3356,6 +3419,7 @@ val memory_rel_Cons = prove(
          GSYM word_add_n2w,WORD_LEFT_ADD_DISTRIB]
   \\ fs [AC STAR_ASSOC STAR_COMM] \\ fs [STAR_ASSOC]
   \\ pop_assum mp_tac \\ CONV_TAC (DEPTH_CONV ETA_CONV)
+  \\ fs [ADD1,GSYM word_add_n2w,WORD_LEFT_ADD_DISTRIB]
   \\ fs [AC STAR_ASSOC STAR_COMM] \\ fs [STAR_ASSOC]);
 
 val get_real_addr_lemma = store_thm("get_real_addr_lemma",
@@ -3395,10 +3459,20 @@ val assign_thm = Q.prove(
      (q = SOME NotEnoughSpace ==> r.ffi = t.ffi) /\
      (q <> SOME NotEnoughSpace ==>
      state_rel c l1 l2 (set_var dest v s2) r [] locs /\ q = NONE)`,
-
   strip_tac \\ drule (evaluate_GiveUp |> GEN_ALL) \\ rw [] \\ fs []
   \\ imp_res_tac state_rel_cut_IMP \\ pop_assum mp_tac
   \\ qpat_assum `state_rel c l1 l2 s t [] locs` kall_tac \\ strip_tac
+  \\ Cases_on `op = Ref` \\ fs [] THEN1
+   (imp_res_tac get_vars_IMP_LENGTH \\ fs []
+    \\ fs [assign_def] \\ fs [do_app] \\ every_case_tac \\ fs []
+    \\ imp_res_tac get_vars_IMP_LENGTH \\ fs [] \\ clean_tac
+    \\ fs [consume_space_def] \\ clean_tac
+    \\ imp_res_tac state_rel_get_vars_IMP
+    \\ fs [state_rel_thm] \\ eval_tac
+    \\ full_simp_tac std_ss [GSYM APPEND_ASSOC]
+    \\ drule (memory_rel_get_vars_IMP |> GEN_ALL)
+    \\ disch_then drule \\ fs [NOT_LESS,DECIDE ``n + 1 <= m <=> n < m:num``]
+    \\ cheat)
   \\ Cases_on `op = Update` \\ fs [] THEN1
    (imp_res_tac get_vars_IMP_LENGTH \\ fs []
     \\ fs [do_app] \\ every_case_tac \\ fs [] \\ clean_tac
@@ -3481,7 +3555,7 @@ val assign_thm = Q.prove(
    (var_eq_tac \\ fs [do_app]
     \\ every_case_tac \\ fs []
     \\ rpt var_eq_tac
-    \\ fs [bvp_to_wordTheory.assign_def]
+    \\ fs [assign_def]
     \\ Cases_on `i` \\ fs []
     \\ fs [wordSemTheory.evaluate_def,wordSemTheory.word_exp_def]
     \\ fs [state_rel_def,wordSemTheory.set_var_def,set_var_def,
@@ -3497,7 +3571,7 @@ val assign_thm = Q.prove(
    (var_eq_tac \\ fs [do_app]
     \\ every_case_tac \\ fs []
     \\ rpt var_eq_tac
-    \\ fs [bvp_to_wordTheory.assign_def]
+    \\ fs [assign_def]
     \\ fs [bvp_to_bvi_def]
     \\ fs[wordSemTheory.evaluate_def,wordSemTheory.word_exp_def]
     \\ fs [state_rel_def]
@@ -3514,7 +3588,7 @@ val assign_thm = Q.prove(
    (var_eq_tac \\ fs [do_app]
     \\ every_case_tac \\ fs []
     \\ rpt var_eq_tac
-    \\ fs [bvp_to_wordTheory.assign_def]
+    \\ fs [assign_def]
     \\ imp_res_tac get_vars_SING \\ fs []
     \\ `args <> []` by (strip_tac \\ fs [bvpSemTheory.get_vars_def])
     \\ fs[wordSemTheory.evaluate_def,wordSemTheory.word_exp_def,Unit_def]
@@ -3541,7 +3615,7 @@ val assign_thm = Q.prove(
   \\ Cases_on `?tag. op = Cons tag` \\ fs [] \\ fs [] THEN1
 
    (Cases_on `LENGTH args = 0` THEN1
-     (fs [bvp_to_wordTheory.assign_def] \\ IF_CASES_TAC \\ fs []
+     (fs [assign_def] \\ IF_CASES_TAC \\ fs []
       \\ fs [LENGTH_NIL] \\ rpt var_eq_tac
       \\ fs [do_app] \\ every_case_tac \\ fs []
       \\ imp_res_tac get_vars_IMP_LENGTH \\ fs []
@@ -3560,7 +3634,7 @@ val assign_thm = Q.prove(
       \\ `n2w (16 * tag + 2) = BlockNil tag : 'a word` by
            fs [BlockNil_def,WORD_MUL_LSL,word_mul_n2w,word_add_n2w]
       \\ fs [cons_thm_EMPTY])
-    \\ fs [bvp_to_wordTheory.assign_def] \\ CASE_TAC \\ fs []
+    \\ fs [assign_def] \\ CASE_TAC \\ fs []
     \\ fs [do_app] \\ every_case_tac \\ fs []
     \\ imp_res_tac get_vars_IMP_LENGTH \\ fs [] \\ clean_tac
     \\ fs [consume_space_def] \\ clean_tac
@@ -3569,12 +3643,7 @@ val assign_thm = Q.prove(
     \\ full_simp_tac std_ss [GSYM APPEND_ASSOC]
     \\ drule (memory_rel_get_vars_IMP |> GEN_ALL)
     \\ disch_then drule \\ fs [NOT_LESS,DECIDE ``n + 1 <= m <=> n < m:num``]
-
-
-
-
     \\ cheat)
-  \\ Cases_on `op = Ref` \\ fs [] THEN1 cheat
   \\ Cases_on `op = ToList` \\ fs [] THEN1 (fs [do_app])
   \\ Cases_on `op = AllocGlobal` \\ fs [] THEN1 (fs [do_app])
   \\ Cases_on `?i. op = Global i` \\ fs [] THEN1 (fs [do_app])
